\begin{eqnarray*}
x ^ 2 +( a ^2 + a)x + a -1 = 0 \\
x + 3 = 0
\end{eqnarray*}

$
\begin{align*}
(-3)^ 2 +( a ^2 + a)(-3) + a -1 = 0 \\
9 - 3(a ^2 + a ) + a -1 = 0 \\
- 3 a ^2 -3a + a  + 8 = 0 \\
- 3 a ^2 -2a + 8 = 0 \\
3a ^ 2 + 2a  - 8 = 0
\end{align*}
$

\begin{equation*}
x = \frac{-b\pm{\sqrt{b^2 - 4ac}}}{2a}
\end{equation*}

$
\begin{align}
x & = \frac{-2\pm{\sqrt{(2)^2 - 4(3\times{ -8})}}}{2\times{3}}ã€€ \\
  & = \frac{-2\pm{\sqrt{4 + 4 \times{ 24}}}}{6} \\
  & = \frac{-2\pm{2\sqrt{1+24}}}{6} \\
  & = \frac{-2\pm{10}}{6} \\
  & = \frac{-12, 8}{6} \\
  & = -2, \frac{4}{3}
\end{align}
$